refactor

DenotSem/Deterministic.thy
@@ -4,139 +4,11 @@ theory Deterministic
 begin
 (*>*)
 
-section "Model is Deterministic, Intersection Intro is Admissible"
+section "Environment Weakening" 
   
-lemma wf_eval: "\<lbrakk> v \<in> \<lbrakk>e\<rbrakk>\<rho>; wf_env \<rho> \<rbrakk> \<Longrightarrow> wf_ty v"
-  apply (induction e) apply (case_tac "x < length \<rho>") apply force+ done
-    
-lemma consis_codomain:
-  fixes a b c d
-  assumes ab_g1: "a\<rightarrow>b \<in> set \<Gamma>1" and cd_g2: "c\<rightarrow>d \<in> set \<Gamma>2" and
-    v1_g1: "\<forall>v v'. v\<rightarrow>v' \<in> set \<Gamma>1 \<longrightarrow> v1 <: v" and
-    v2_g2: "\<forall>v v'. v\<rightarrow>v' \<in> set \<Gamma>2 \<longrightarrow> v2 <: v" and
-    v1_v2: "v1 ~ v2" and f1_f2: "f1 ~ f2" and
-    g1_f1: "set \<Gamma>1 \<subseteq> atoms f1" and g2_f2: "set \<Gamma>2 \<subseteq> atoms f2"
-  shows "b ~ d"
-proof -    
-    have v1_a: "v1 <: a" using v1_g1 ab_g1 by blast 
-    have v2_c: "v2 <: c" using v2_g2 cd_g2 by blast
-    have a_c: "a ~ c" using v1_a v2_c v1_v2 consis_le by blast        
-    have ab_cd: "a\<rightarrow>b ~ c\<rightarrow>d"
-      using ab_g1 cd_g2 g1_f1 g2_f2 f1_f2 consis_atoms by blast
-    show "b ~ d" using ab_cd a_c by simp 
-qed
-
-    
-lemma all_fun_ex: "\<lbrakk> all_funs (set \<Gamma>); x \<in> set \<Gamma>; \<And> a b. \<lbrakk> x = a \<rightarrow> b \<rbrakk> \<Longrightarrow> P \<rbrakk> \<Longrightarrow> P"
-  apply (cases x) apply auto done
-
-lemma all_fun_ex_dom: "\<lbrakk> all_funs (set \<Gamma>); y \<in> set (map cod \<Gamma>) \<rbrakk> \<Longrightarrow> \<exists>x. x\<rightarrow>y \<in> set \<Gamma>"
-  apply (induction \<Gamma> arbitrary: y)
-  apply force
-  apply simp apply (erule disjE) 
-   apply simp apply (case_tac a) apply force apply force apply force
-  apply blast
-  done
-    
-lemma consistent_app: assumes f1_f2: "f1 ~ f2" and v1_v2: "v1 ~ v2" and 
-  f1_v1: "v1' \<in> f1 \<bullet> v1"  and f2_v2: "v2' \<in> f2 \<bullet> v2" and
-  wf_f1: "wf_ty f1" and wf_f2: "wf_ty f2" and wf_v1: "wf_ty v1" and wf_v2: "wf_ty v2"
-shows "v1' ~ v2'"
-proof -
-  have f1_v11: "f1 <: v1 \<rightarrow> v1'" using f1_v1 by simp
-  have f2_v22: "f2 <: v2 \<rightarrow> v2'" using f2_v2 by simp
-      
-  obtain \<Gamma>1 where g1_ne: "\<Gamma>1 \<noteq> []" and af_g1: "all_funs (set \<Gamma>1)" and g1_f1: "set \<Gamma>1 \<subseteq> atoms f1" and
-    v1_g1: "\<forall>v v'. v\<rightarrow>v' \<in> set \<Gamma>1 \<longrightarrow> v1 <: v" and g1_v1p: "\<Sqinter>(map cod \<Gamma>1) <: v1'"
-    using f1_v11 sub_fun_any_inv_atoms[of f1 v1 v1'] by blast
-  let ?C1 = "map cod \<Gamma>1"     
-  obtain \<Gamma>2 where g2_ne: "\<Gamma>2 \<noteq> []" and af_g2: "all_funs (set \<Gamma>2)" and g2_f2: "set \<Gamma>2 \<subseteq> atoms f2" and
-    v2_g2: "\<forall>v v'. v\<rightarrow>v' \<in> set \<Gamma>2 \<longrightarrow> v2 <: v" and g2_v2p: "\<Sqinter>(map cod \<Gamma>2) <: v2'"
-    using f2_v22 sub_fun_any_inv_atoms[of f2 v2 v2'] by blast
-  let ?C2 = "map cod \<Gamma>2"
-
-  have wf_c1: "\<forall>v. v \<in> set ?C1 \<longrightarrow> wf_ty v"
-    using g1_f1 wf_f1 af_g1 apply auto
-    apply (erule all_fun_ex) apply blast apply simp using wf_atoms apply auto done
-  have wf_c2: "\<forall>v. v \<in> set ?C2 \<longrightarrow> wf_ty v"
-    using g2_f2 wf_f2 af_g2 apply auto
-    apply (erule all_fun_ex) apply blast apply simp using wf_atoms apply auto done
-  have c_c1: "\<forall>v1' v2'. {v1',v2'} \<subseteq> set ?C1 \<longrightarrow> v1' ~ v2'"
-  proof clarify
-    fix v1' v2' assume 1: "{v1',v2'} \<subseteq> set ?C1"        
-    have v1_c1: "v1' \<in> set ?C1" using 1 by blast 
-    have v2_c1: "v2' \<in> set ?C1" using 1 by blast
-    obtain d1 where v11_g1: "d1\<rightarrow>v1' \<in> set \<Gamma>1" using v1_c1 af_g1 all_fun_ex_dom[of \<Gamma>1 v1'] by blast
-    obtain d2 where v22_g1: "d2\<rightarrow>v2' \<in> set \<Gamma>1" using v2_c1 af_g1 all_fun_ex_dom[of \<Gamma>1 v2'] by blast        
-    show "v1' ~ v2'"
-      apply (rule consis_codomain[of d1 v1' \<Gamma>1 d2 v2' \<Gamma>1 v1 v1 f1 f1])
-      using v11_g1 v22_g1 v1_g1 consis_refl wf_v1 wf_f1 g1_f1 by auto   
-  qed
-  have c_c2: "\<forall>v1' v2'. {v1',v2'} \<subseteq> set ?C2 \<longrightarrow> v1' ~ v2'"
-  proof clarify
-    fix v1' v2' assume 1: "{v1',v2'} \<subseteq> set ?C2"        
-    have v1_c1: "v1' \<in> set ?C2" using 1 by blast 
-    have v2_c1: "v2' \<in> set ?C2" using 1 by blast
-    obtain d1 where v11_g2: "d1\<rightarrow>v1' \<in> set \<Gamma>2" using v1_c1 af_g2 all_fun_ex_dom[of \<Gamma>2 v1'] by blast
-    obtain d2 where v22_g2: "d2\<rightarrow>v2' \<in> set \<Gamma>2" using v2_c1 af_g2 all_fun_ex_dom[of \<Gamma>2 v2'] by blast        
-    show "v1' ~ v2'"
-      apply (rule consis_codomain[of d1 v1' \<Gamma>2 d2 v2' \<Gamma>2 v2 v2 f2 f2])
-      using v11_g2 v22_g2 v2_g2 consis_refl wf_v2 wf_f2 g2_f2 by auto   
-  qed
-  have c1_c2: "\<Sqinter>?C1 ~ \<Sqinter>?C2" 
-  proof (rule meet_list_consis)
-    show "map cod \<Gamma>1 \<noteq> []" using g1_ne by auto
-  next
-    show "map cod \<Gamma>2 \<noteq> []" using g2_ne by auto
-  next
-    show "\<forall>v1 v2. {v1, v2} \<subseteq> set ?C1 \<union> set ?C2 \<longrightarrow> v1 ~ v2"
-    proof clarify
-      fix v1' v2' assume 1: "{v1',v2'} \<subseteq> set ?C1 \<union> set ?C2"        
-      { assume v1_c1: "v1' \<in> set ?C1" and v2_c1: "v2' \<in> set ?C1"
-        have "v1' ~ v2'" using v1_c1 v2_c1 c_c1 by blast
-      } moreover {
-        assume v1_c1: "v1' \<in> set ?C1" and v2_c2: "v2' \<in> set ?C2"
-        obtain d1 where v11_g1: "d1\<rightarrow>v1' \<in> set \<Gamma>1" using v1_c1 af_g1 all_fun_ex_dom[of \<Gamma>1 v1'] by blast
-        obtain d2 where v22_g2: "d2\<rightarrow>v2' \<in> set \<Gamma>2" using v2_c2 af_g2 all_fun_ex_dom[of \<Gamma>2 v2'] by blast        
-        have "v1' ~ v2'" 
-          apply (rule consis_codomain)
-          using v11_g1 apply blast using v22_g2 apply blast using v1_g1 apply blast
-          using v2_g2 apply blast using v1_v2 apply blast using f1_f2 apply blast
-          using g1_f1 apply blast using g2_f2 apply blast done          
-      } moreover {
-        assume v1_c2: "v1' \<in> set ?C2" and v2_c1: "v2' \<in> set ?C1"
-        obtain d1 where v11_g2: "d1\<rightarrow>v1' \<in> set \<Gamma>2" using v1_c2 af_g2 all_fun_ex_dom[of \<Gamma>2 v1'] by blast
-        obtain d2 where v22_g1: "d2\<rightarrow>v2' \<in> set \<Gamma>1" using v2_c1 af_g1 all_fun_ex_dom[of \<Gamma>1 v2'] by blast        
-        have "v1' ~ v2'" 
-          apply (rule consis_codomain)
-          using v11_g2 apply blast using v22_g1 apply blast using v2_g2 apply blast
-          using v1_g1 apply blast using v1_v2 consis_sym apply blast
-          apply (rule consis_sym) using f1_f2 apply blast using g2_f2 apply blast           
-          using g1_f1 apply blast done        
-      } moreover {
-        assume v1_c2: "v1' \<in> set ?C2" and v2_c2: "v2' \<in> set ?C2"
-        have "v1' ~ v2'" using v1_c2 v2_c2 c_c2 g2_ne by auto 
-      } ultimately show "v1' ~ v2'" using 1 by blast
-    qed      
-  qed  
-  then show ?thesis using g1_v1p g2_v2p consis_le by blast
-qed
-
-lemma inter_app: assumes f1_v1: "v1' \<in> f1 \<bullet> v1" and f2_v2: "v2' \<in> f2 \<bullet> v2" and 
-  f1_f2: "f1 ~ f2" and v1_v2: "v1 ~ v2" and v1p_v2p: "v1' ~ v2'"
-  shows "v1' \<sqinter> v2' \<in> (f1 \<sqinter> f2) \<bullet> (v1 \<sqinter> v2)"
-proof -
-  have wf_v12: "wf_ty (v1' \<sqinter> v2')" using f1_v1 f2_v2 v1p_v2p by auto 
-  have f1_v1p: "f1 <: v1 \<rightarrow> v1'" using f1_v1 by simp
-  have f2_v2p: "f2 <: v2 \<rightarrow> v2'" using f2_v2 by simp  
-  have "f1 \<sqinter> f2 <: (v1\<rightarrow>v1') \<sqinter> (v2\<rightarrow>v2')" using f1_v1p f2_v2p by (rule sub_mon)
-  also have "(v1 \<rightarrow> v1') \<sqinter> (v2 \<rightarrow> v2') <: (v1 \<sqinter> v2) \<rightarrow> (v1' \<sqinter> v2')" by (rule sub_dist_union_fun)
-  finally have "f1 \<sqinter> f2 <: (v1 \<sqinter> v2) \<rightarrow> (v1' \<sqinter> v2')" using sub_trans by auto
-  then show ?thesis using wf_v12 by simp
-qed
-
-lemma weaken_env_fun_aux: "\<lbrakk> F v e \<rho>1; \<rho>2 <: \<rho>1; (\<forall> v \<rho>1 \<rho>2. v \<in> \<lbrakk>e\<rbrakk>\<rho>1 \<longrightarrow> \<rho>2 <: \<rho>1 \<longrightarrow> v \<in> \<lbrakk>e\<rbrakk>\<rho>2) \<rbrakk>
-                    \<Longrightarrow> F v e \<rho>2"
+lemma weaken_env_fun_aux: 
+  "\<lbrakk> F v e \<rho>1; \<rho>2 <: \<rho>1; (\<forall> v \<rho>1 \<rho>2. v \<in> \<lbrakk>e\<rbrakk>\<rho>1 \<longrightarrow> \<rho>2 <: \<rho>1 \<longrightarrow> v \<in> \<lbrakk>e\<rbrakk>\<rho>2) \<rbrakk>
+   \<Longrightarrow> F v e \<rho>2"
 proof (induction v arbitrary: e \<rho>1 \<rho>2)
   case (TNat n)
   then have "False" by auto
@@ -175,8 +47,151 @@ qed
 lemma weaken_env_fun: "\<lbrakk> F v e \<rho>1; \<rho>2 <: \<rho>1 \<rbrakk> \<Longrightarrow> F v e \<rho>2"
   using weaken_env_fun_aux weaken_env by blast
 
-lemma denot_fun_atoms: "\<lbrakk> all_funs (atoms v); \<forall>v1 v2. v1\<rightarrow>v2 \<in> atoms v \<longrightarrow> v2 \<in> \<lbrakk>e\<rbrakk>v1#\<rho> \<rbrakk>
-   \<Longrightarrow> F v e \<rho>"
+
+section "Determinism and Admissability of Intersection Intro"
+  
+lemma wf_eval: "\<lbrakk> v \<in> \<lbrakk>e\<rbrakk>\<rho>; wf_env \<rho> \<rbrakk> \<Longrightarrow> wf_ty v"
+  apply (induction e) apply (case_tac "x < length \<rho>") apply force+ done
+    
+lemma consis_codomain:
+  fixes a b c d
+  assumes ab_g1: "a\<rightarrow>b \<in> set \<Gamma>1" and cd_g2: "c\<rightarrow>d \<in> set \<Gamma>2" and
+    v1_g1: "\<forall>v v'. v\<rightarrow>v' \<in> set \<Gamma>1 \<longrightarrow> v1 <: v" and
+    v2_g2: "\<forall>v v'. v\<rightarrow>v' \<in> set \<Gamma>2 \<longrightarrow> v2 <: v" and
+    v1_v2: "v1 ~ v2" and f1_f2: "f1 ~ f2" and
+    g1_f1: "set \<Gamma>1 \<subseteq> atoms f1" and g2_f2: "set \<Gamma>2 \<subseteq> atoms f2"
+  shows "b ~ d"
+proof -    
+    have v1_a: "v1 <: a" using v1_g1 ab_g1 by blast 
+    have v2_c: "v2 <: c" using v2_g2 cd_g2 by blast
+    have a_c: "a ~ c" using v1_a v2_c v1_v2 consis_le by blast        
+    have ab_cd: "a\<rightarrow>b ~ c\<rightarrow>d"
+      using ab_g1 cd_g2 g1_f1 g2_f2 f1_f2 consis_atoms by blast
+    show "b ~ d" using ab_cd a_c by simp 
+qed
+    
+lemma all_fun_ex: "\<lbrakk> all_funs (set \<Gamma>); x \<in> set \<Gamma>; \<And> a b. \<lbrakk> x = a \<rightarrow> b \<rbrakk> \<Longrightarrow> P \<rbrakk> \<Longrightarrow> P"
+  apply (cases x) apply auto done
+
+lemma all_fun_ex_dom: "\<lbrakk> all_funs (set \<Gamma>); y \<in> set (map cod \<Gamma>) \<rbrakk> \<Longrightarrow> \<exists>x. x\<rightarrow>y \<in> set \<Gamma>"
+  apply (induction \<Gamma> arbitrary: y)
+  apply force
+  apply simp apply (erule disjE) 
+   apply simp apply (case_tac a) apply force apply force apply force
+  apply blast
+  done
+    
+lemma consistent_app: assumes f1_f2: "f1 ~ f2" and v1_v2: "v1 ~ v2" and 
+  f1_v1: "v1' \<in> f1 \<bullet> v1"  and f2_v2: "v2' \<in> f2 \<bullet> v2" and
+  wf_f1: "wf_ty f1" and wf_f2: "wf_ty f2" and wf_v1: "wf_ty v1" and wf_v2: "wf_ty v2"
+shows "v1' ~ v2'"
+proof -
+  have f1_v11: "f1 <: v1 \<rightarrow> v1'" using f1_v1 by simp
+  have f2_v22: "f2 <: v2 \<rightarrow> v2'" using f2_v2 by simp
+      
+  obtain \<Gamma>1 where g1_ne: "\<Gamma>1 \<noteq> []" and af_g1: "all_funs (set \<Gamma>1)" and 
+    g1_f1: "set \<Gamma>1 \<subseteq> atoms f1" and
+    v1_g1: "\<forall>v v'. v\<rightarrow>v' \<in> set \<Gamma>1 \<longrightarrow> v1 <: v" and 
+    g1_v1p: "\<Sqinter>(map cod \<Gamma>1) <: v1'"
+    using f1_v11 sub_fun_any_inv_atoms[of f1 v1 v1'] by blast
+  let ?C1 = "map cod \<Gamma>1"     
+  obtain \<Gamma>2 where g2_ne: "\<Gamma>2 \<noteq> []" and af_g2: "all_funs (set \<Gamma>2)" and 
+    g2_f2: "set \<Gamma>2 \<subseteq> atoms f2" and
+    v2_g2: "\<forall>v v'. v\<rightarrow>v' \<in> set \<Gamma>2 \<longrightarrow> v2 <: v" and 
+    g2_v2p: "\<Sqinter>(map cod \<Gamma>2) <: v2'"
+    using f2_v22 sub_fun_any_inv_atoms[of f2 v2 v2'] by blast
+  let ?C2 = "map cod \<Gamma>2"
+
+  have wf_c1: "\<forall>v. v \<in> set ?C1 \<longrightarrow> wf_ty v"
+    using g1_f1 wf_f1 af_g1 apply auto
+    apply (erule all_fun_ex) apply blast apply simp using wf_atoms apply auto done
+  have wf_c2: "\<forall>v. v \<in> set ?C2 \<longrightarrow> wf_ty v"
+    using g2_f2 wf_f2 af_g2 apply auto
+    apply (erule all_fun_ex) apply blast apply simp using wf_atoms apply auto done
+  have c_c1: "\<forall>v1' v2'. {v1',v2'} \<subseteq> set ?C1 \<longrightarrow> v1' ~ v2'"
+  proof clarify
+    fix v1' v2' assume 1: "{v1',v2'} \<subseteq> set ?C1"        
+    have v1_c1: "v1' \<in> set ?C1" using 1 by blast 
+    have v2_c1: "v2' \<in> set ?C1" using 1 by blast
+    obtain d1 where v11_g1: "d1\<rightarrow>v1' \<in> set \<Gamma>1" 
+      using v1_c1 af_g1 all_fun_ex_dom[of \<Gamma>1 v1'] by blast
+    obtain d2 where v22_g1: "d2\<rightarrow>v2' \<in> set \<Gamma>1" 
+      using v2_c1 af_g1 all_fun_ex_dom[of \<Gamma>1 v2'] by blast        
+    show "v1' ~ v2'"
+      apply (rule consis_codomain[of d1 v1' \<Gamma>1 d2 v2' \<Gamma>1 v1 v1 f1 f1])
+      using v11_g1 v22_g1 v1_g1 consis_refl wf_v1 wf_f1 g1_f1 by auto   
+  qed
+  have c_c2: "\<forall>v1' v2'. {v1',v2'} \<subseteq> set ?C2 \<longrightarrow> v1' ~ v2'"
+  proof clarify
+    fix v1' v2' assume 1: "{v1',v2'} \<subseteq> set ?C2"        
+    have v1_c1: "v1' \<in> set ?C2" using 1 by blast 
+    have v2_c1: "v2' \<in> set ?C2" using 1 by blast
+    obtain d1 where v11_g2: "d1\<rightarrow>v1' \<in> set \<Gamma>2" 
+      using v1_c1 af_g2 all_fun_ex_dom[of \<Gamma>2 v1'] by blast
+    obtain d2 where v22_g2: "d2\<rightarrow>v2' \<in> set \<Gamma>2" 
+      using v2_c1 af_g2 all_fun_ex_dom[of \<Gamma>2 v2'] by blast        
+    show "v1' ~ v2'"
+      apply (rule consis_codomain[of d1 v1' \<Gamma>2 d2 v2' \<Gamma>2 v2 v2 f2 f2])
+      using v11_g2 v22_g2 v2_g2 consis_refl wf_v2 wf_f2 g2_f2 by auto   
+  qed
+  have c1_c2: "\<Sqinter>?C1 ~ \<Sqinter>?C2" 
+  proof (rule meet_list_consis)
+    show "map cod \<Gamma>1 \<noteq> []" using g1_ne by auto
+  next
+    show "map cod \<Gamma>2 \<noteq> []" using g2_ne by auto
+  next
+    show "\<forall>v1 v2. {v1, v2} \<subseteq> set ?C1 \<union> set ?C2 \<longrightarrow> v1 ~ v2"
+    proof clarify
+      fix v1' v2' assume 1: "{v1',v2'} \<subseteq> set ?C1 \<union> set ?C2"        
+      { assume v1_c1: "v1' \<in> set ?C1" and v2_c1: "v2' \<in> set ?C1"
+        have "v1' ~ v2'" using v1_c1 v2_c1 c_c1 by blast
+      } moreover {
+        assume v1_c1: "v1' \<in> set ?C1" and v2_c2: "v2' \<in> set ?C2"
+        obtain d1 where v11_g1: "d1\<rightarrow>v1' \<in> set \<Gamma>1" 
+          using v1_c1 af_g1 all_fun_ex_dom[of \<Gamma>1 v1'] by blast
+        obtain d2 where v22_g2: "d2\<rightarrow>v2' \<in> set \<Gamma>2" 
+          using v2_c2 af_g2 all_fun_ex_dom[of \<Gamma>2 v2'] by blast        
+        have "v1' ~ v2'" 
+          apply (rule consis_codomain)
+          using v11_g1 apply blast using v22_g2 apply blast using v1_g1 apply blast
+          using v2_g2 apply blast using v1_v2 apply blast using f1_f2 apply blast
+          using g1_f1 apply blast using g2_f2 apply blast done          
+      } moreover {
+        assume v1_c2: "v1' \<in> set ?C2" and v2_c1: "v2' \<in> set ?C1"
+        obtain d1 where v11_g2: "d1\<rightarrow>v1' \<in> set \<Gamma>2" 
+          using v1_c2 af_g2 all_fun_ex_dom[of \<Gamma>2 v1'] by blast
+        obtain d2 where v22_g1: "d2\<rightarrow>v2' \<in> set \<Gamma>1" 
+          using v2_c1 af_g1 all_fun_ex_dom[of \<Gamma>1 v2'] by blast        
+        have "v1' ~ v2'" 
+          apply (rule consis_codomain)
+          using v11_g2 apply blast using v22_g1 apply blast using v2_g2 apply blast
+          using v1_g1 apply blast using v1_v2 consis_sym apply blast
+          apply (rule consis_sym) using f1_f2 apply blast using g2_f2 apply blast           
+          using g1_f1 apply blast done        
+      } moreover {
+        assume v1_c2: "v1' \<in> set ?C2" and v2_c2: "v2' \<in> set ?C2"
+        have "v1' ~ v2'" using v1_c2 v2_c2 c_c2 g2_ne by auto 
+      } ultimately show "v1' ~ v2'" using 1 by blast
+    qed      
+  qed  
+  then show ?thesis using g1_v1p g2_v2p consis_le by blast
+qed
+
+lemma inter_app: assumes f1_v1: "v1' \<in> f1 \<bullet> v1" and f2_v2: "v2' \<in> f2 \<bullet> v2" and 
+  f1_f2: "f1 ~ f2" and v1_v2: "v1 ~ v2" and v1p_v2p: "v1' ~ v2'"
+  shows "v1' \<sqinter> v2' \<in> (f1 \<sqinter> f2) \<bullet> (v1 \<sqinter> v2)"
+proof -
+  have wf_v12: "wf_ty (v1' \<sqinter> v2')" using f1_v1 f2_v2 v1p_v2p by auto 
+  have f1_v1p: "f1 <: v1 \<rightarrow> v1'" using f1_v1 by simp
+  have f2_v2p: "f2 <: v2 \<rightarrow> v2'" using f2_v2 by simp  
+  have "f1 \<sqinter> f2 <: (v1\<rightarrow>v1') \<sqinter> (v2\<rightarrow>v2')" using f1_v1p f2_v2p by (rule sub_mon)
+  also have "(v1 \<rightarrow> v1') \<sqinter> (v2 \<rightarrow> v2') <: (v1 \<sqinter> v2) \<rightarrow> (v1' \<sqinter> v2')" by (rule sub_dist_union_fun)
+  finally have "f1 \<sqinter> f2 <: (v1 \<sqinter> v2) \<rightarrow> (v1' \<sqinter> v2')" using sub_trans by auto
+  then show ?thesis using wf_v12 by simp
+qed
+
+lemma denot_fun_atoms: 
+  "\<lbrakk> all_funs (atoms v); \<forall>v1 v2. v1\<rightarrow>v2 \<in> atoms v \<longrightarrow> v2 \<in> \<lbrakk>e\<rbrakk>v1#\<rho> \<rbrakk> \<Longrightarrow> F v e \<rho>"
   by (induction v) auto    
 
 lemma denot_fun_inv_atoms: "F v e \<rho> \<Longrightarrow> all_funs (atoms v) 
@@ -186,35 +201,6 @@ lemma denot_fun_inv_atoms: "F v e \<rho> \<Longrightarrow> all_funs (atoms v)
 lemma eval_fun_all_funs: "F v e \<rho> \<Longrightarrow> all_funs (atoms v)"
   apply (induction v) apply auto done
 
-abbreviation subsump :: "ty \<Rightarrow> ty \<Rightarrow> exp \<Rightarrow> ty list \<Rightarrow> bool" where
-  "subsump v1 v2 e \<rho> \<equiv> v1 \<in> \<lbrakk>e\<rbrakk>\<rho> \<longrightarrow> v1 <: v2 \<longrightarrow> wf_ty v2 \<longrightarrow> wf_env \<rho> \<longrightarrow> v2 \<in> \<lbrakk>e\<rbrakk>\<rho>" 
-
-abbreviation determ :: "ty \<Rightarrow> ty \<Rightarrow> exp \<Rightarrow> ty list \<Rightarrow> ty list \<Rightarrow> bool" where
-  "determ v1 v2 e \<rho>1 \<rho>2 \<equiv> v1\<in> \<lbrakk>e\<rbrakk>\<rho>1 \<longrightarrow> v2\<in> \<lbrakk>e\<rbrakk>\<rho>2 \<longrightarrow> wf_env \<rho>1 \<longrightarrow> wf_env \<rho>2 \<longrightarrow> consis_env \<rho>1 \<rho>2
-    \<longrightarrow> v1 \<sqinter> v2 \<in> \<lbrakk>e\<rbrakk>(\<rho>1\<sqinter>\<rho>2) \<and> wf_ty (v1 \<sqinter> v2)"
-
-lemma fun_eval_distr_determ:
-  "\<lbrakk> F (A \<rightarrow> B \<sqinter> C \<rightarrow> D) e \<rho>; \<forall>v1 v2 \<rho>1 \<rho>2. determ v1 v2 e \<rho>1 \<rho>2; wf_env \<rho>; wf_ty A; wf_ty C; A ~ C \<rbrakk>
-    \<Longrightarrow> F ((A \<sqinter> C) \<rightarrow> (B \<sqinter> D)) e \<rho>"
-  apply simp apply clarify
-  apply (subgoal_tac "(A\<sqinter>C)#\<rho> <: A # \<rho>") prefer 2 apply simp 
-   apply clarify apply (case_tac k) apply force apply force
-  apply (subgoal_tac "(A\<sqinter>C)#\<rho> <: C # \<rho>") prefer 2 apply simp 
-   apply clarify apply (case_tac k) apply force apply force
-  apply (subgoal_tac "B \<in> \<lbrakk>e\<rbrakk>(A\<sqinter>C)#\<rho>") prefer 2 using weaken_env apply blast
-  apply (subgoal_tac "D \<in> \<lbrakk>e\<rbrakk>(A\<sqinter>C)#\<rho>") prefer 2 using weaken_env apply blast
-  apply (subgoal_tac "wf_env ((A\<sqinter>C)#\<rho>)") prefer 2 apply simp apply clarify
-    apply (case_tac k) apply simp apply blast apply force
-  apply (subgoal_tac "B \<sqinter> D \<in> \<lbrakk>e\<rbrakk>((A \<sqinter> C) # \<rho>) \<sqinter> ((A \<sqinter> C) # \<rho>)") prefer 2 apply blast
-  apply (subgoal_tac "(A \<sqinter> C) # \<rho> <: ((A \<sqinter> C) # \<rho>) \<sqinter> ((A \<sqinter> C) # \<rho>)") prefer 2
-   apply simp apply clarify apply (case_tac k) prefer 2 apply force
-    apply simp 
-  apply blast
-  apply (rule weaken_env)    
-   apply blast
-    apply blast
-  done
- 
 lemma denot_fold_meet_inv_init: "F (fold op \<sqinter> L A) e \<rho> \<Longrightarrow> F A e \<rho>"
   apply (induction L arbitrary: A)
    apply force
@@ -237,11 +223,190 @@ abbreviation consis_funs :: "ty list \<Rightarrow> bool" where
 
 abbreviation wf_list :: "ty list \<Rightarrow> bool" where
   "wf_list L \<equiv> \<forall>v. v \<in> set L \<longrightarrow> wf_ty v"
+
+abbreviation determ :: "ty \<Rightarrow> ty \<Rightarrow> exp \<Rightarrow> ty list \<Rightarrow> ty list \<Rightarrow> bool" where
+  "determ v1 v2 e \<rho>1 \<rho>2 \<equiv> v1 \<in> \<lbrakk>e\<rbrakk>\<rho>1 \<longrightarrow> v2 \<in> \<lbrakk>e\<rbrakk>\<rho>2
+     \<longrightarrow> wf_env \<rho>1 \<longrightarrow> wf_env \<rho>2 \<longrightarrow> consis_env \<rho>1 \<rho>2
+     \<longrightarrow> v1 \<sqinter> v2 \<in> \<lbrakk>e\<rbrakk>(\<rho>1\<sqinter>\<rho>2) \<and> wf_ty (v1 \<sqinter> v2)" 
  
+lemma deterministic: "\<forall> v1 v2 \<rho>1 \<rho>2. determ v1 v2 e \<rho>1 \<rho>2"
+proof (induction e)
+  case (EVar x)
+  show ?case
+    apply clarify
+    apply (case_tac "x < length \<rho>1") defer apply force
+    using consis_le inter_func by auto
+next
+  case (ENat n)
+  then show ?case 
+    by  (auto simp: consis_le inter_func)      
+next
+  case (ELam e)
+  show ?case
+    apply (rule allI)+ apply (rule impI)+
+  proof -
+    fix v1 v2 \<rho>1 \<rho>2 assume v1_le: "v1 \<in> \<lbrakk>\<lambda> e\<rbrakk>\<rho>1" and v2_le: "v2 \<in> \<lbrakk>\<lambda> e\<rbrakk>\<rho>2" and
+      wf_r1: "wf_env \<rho>1" and wf_r2: "wf_env \<rho>2" and c_r1_r2: "consis_env \<rho>1 \<rho>2" 
+    have wf_v1: "wf_ty v1" using v1_le by simp
+    have wf_v2: "wf_ty v2" using v2_le by simp
+    have f_v1_e_r1: "F v1 e \<rho>1" using v1_le by simp      
+    have f_v2_e_r2: "F v2 e \<rho>2" using v2_le by simp      
+    have r12_r1: "\<rho>1\<sqinter>\<rho>2 <: \<rho>1" using c_r1_r2 by auto
+    have r12_r2: "\<rho>1\<sqinter>\<rho>2 <: \<rho>2" using c_r1_r2 by auto
+    have "v1 ~ v2" apply (rule atoms_consis) apply clarify
+    proof -
+      fix A1 A2 assume a1_v1: "A1 \<in> atoms v1" and a2_v2: "A2 \<in> atoms v2"
+      obtain A11 A12 where a1: "A1=A11\<rightarrow>A12" and a12_e: "A12 \<in> \<lbrakk>e\<rbrakk>A11#\<rho>1" using f_v1_e_r1 
+        by (metis a1_v1 atoms_not_inter denot_fun_inv_atoms ty.simps(10)
+            wf_atoms wf_ty.simps wf_v1)
+      obtain A21 A22 where a2: "A2=A21\<rightarrow>A22" and a22_e: "A22 \<in> \<lbrakk>e\<rbrakk>A21#\<rho>2" using f_v2_e_r2 
+        by (metis a2_v2 atoms_not_inter denot_fun_inv_atoms ty.simps(10) 
+            wf_atoms wf_ty.simps wf_v2)
+      show "A1 ~ A2"
+      proof (cases "A11 ~ A21")
+        case True
+        have c_ar1_ar2: "consis_env (A11#\<rho>1) (A21#\<rho>2)" using True c_r1_r2 apply auto
+          apply (case_tac k) apply auto done
+        have wf_ar1: "wf_env (A11#\<rho>1)" using wf_r1 a1 a1_v1 wf_v1 apply auto
+          apply (case_tac k) apply auto using wf_ty_arrow_inv by blast
+        have wf_ar2: "wf_env (A21#\<rho>2)" using wf_r2 a2 a2_v2 wf_v2 apply auto
+          apply (case_tac k) apply auto using wf_ty_arrow_inv by blast
+        have "determ A12 A22 e (A11#\<rho>1) (A21#\<rho>2)" using ELam by blast
+        then show ?thesis using c_ar1_ar2 a12_e a22_e wf_ar1 wf_ar2 True a1 a2 by auto
+      next
+        case False
+        then show ?thesis using a1 a2 by simp
+      qed
+    qed        
+    then have wf_v12: "wf_ty (v1 \<sqinter> v2)" using wf_v1 wf_v2 by auto
+    have f_v1_e: "F v1 e (\<rho>1 \<sqinter> \<rho>2)" using f_v1_e_r1 r12_r1 weaken_env_fun by blast
+    have f_v2_e: "F v2 e (\<rho>1 \<sqinter> \<rho>2)" using f_v2_e_r2 r12_r2 weaken_env_fun by blast
+    show "v1 \<sqinter> v2 \<in> \<lbrakk>\<lambda> e\<rbrakk>\<rho>1 \<sqinter> \<rho>2 \<and> wf_ty (v1 \<sqinter> v2)" using wf_v12 f_v1_e f_v2_e by simp
+  qed
+next
+  case (EApp e1 e2)
+  show ?case
+    apply (rule allI)+ apply (rule impI)+
+  proof -
+    fix v1 v2 \<rho>1 \<rho>2 assume v1_e1e2: "v1 \<in> \<lbrakk>EApp e1 e2\<rbrakk>\<rho>1" and v2_e1e2: "v2 \<in> \<lbrakk>EApp e1 e2\<rbrakk>\<rho>2" and
+      wf_r1: "wf_env \<rho>1" and wf_r2: "wf_env \<rho>2" and c_r1_r2: "consis_env \<rho>1 \<rho>2"
+    obtain f1 v21 where f1_e1: "f1 \<in> \<lbrakk>e1\<rbrakk>\<rho>1" and v21_e2: "v21\<in> \<lbrakk>e2\<rbrakk>\<rho>1" and 
+      f1_v21: "v1 \<in> f1 \<bullet> v21" using v1_e1e2 by auto
+    obtain f2 v22 where f2_e1: "f2 \<in> \<lbrakk>e1\<rbrakk>\<rho>2" and v22_e2: "v22\<in> \<lbrakk>e2\<rbrakk>\<rho>2" and 
+      f2_v22: "v2 \<in> f2 \<bullet> v22" using v2_e1e2 by auto
+    have "determ f1 f2 e1 \<rho>1 \<rho>2" using EApp(1) by blast
+    then have f12_e1: "f1 \<sqinter> f2 \<in> \<lbrakk>e1\<rbrakk>\<rho>1\<sqinter>\<rho>2" and wf_f12: "wf_ty (f1 \<sqinter> f2)"         
+      using f1_e1 f2_e1 wf_r1 wf_r2 c_r1_r2 by auto
+    have "determ v21 v22 e2 \<rho>1 \<rho>2" using EApp(2) by blast
+    then have v22_e2: "v21 \<sqinter> v22 \<in> \<lbrakk>e2\<rbrakk>\<rho>1\<sqinter>\<rho>2" and wf_v21_v22: "wf_ty (v21 \<sqinter> v22)"
+      using v21_e2 v22_e2 wf_r1 wf_r2 c_r1_r2 by auto
+    have f12_v21_v22: "v1 \<sqinter> v2 \<in> (f1 \<sqinter> f2) \<bullet> (v21 \<sqinter> v22)"
+      using inter_app[of v1 f1 v21 v2 f2 v22] f1_v21 f2_v22 wf_f12 wf_v21_v22 
+      by (metis CollectD consis_le consistent.simps(4) wf_ty_inter_inv)
+    have v1_v2: "v1 ~ v2"
+      using consistent_app[of f1 f2 v21 v22 v1 v2] wf_f12 wf_v21_v22 f1_v21 f2_v22 by blast
+    have wf_v1: "wf_ty v1" using f1_v21 by blast
+    have wf_v2: "wf_ty v2" using f2_v22 by blast
+    show "v1 \<sqinter> v2 \<in> \<lbrakk>EApp e1 e2\<rbrakk>\<rho>1 \<sqinter> \<rho>2 \<and> wf_ty (v1 \<sqinter> v2)"
+      using f12_e1 v22_e2 v1_v2 wf_v1 wf_v2 v1_v2 f12_v21_v22 by auto
+  qed      
+next
+  case (EPrim f e1 e2)
+  show ?case 
+    apply (rule allI)+ apply (rule impI)+
+  proof -
+    fix v1 v2 \<rho>1 \<rho>2
+    assume v1_p: "v1 \<in> \<lbrakk>EPrim f e1 e2\<rbrakk>\<rho>1" and v2_p: "v2 \<in> \<lbrakk>EPrim f e1 e2\<rbrakk>\<rho>2" and 
+      wf_r1: "wf_env \<rho>1" and wf_r2: "wf_env \<rho>2" and c_r1_r2: "consis_env \<rho>1 \<rho>2"
+    obtain v11 v21 n1 n2 where v11_e1_r1: "v11 \<in> \<lbrakk>e1\<rbrakk>\<rho>1" and v21_e2_r1: "v21 \<in> \<lbrakk>e2\<rbrakk>\<rho>1" and
+      v11_n1: "v11 <: TNat n1" and v21_n2: "v21 <: TNat n2" and
+      fn12_v1: "TNat (f n1 n2) <: v1" and wf_v1: "wf_ty v1" using v1_p by auto
+    obtain v12 v22 n3 n4 where v12_e1_r2: "v12 \<in> \<lbrakk>e1\<rbrakk>\<rho>2" and v22_e2_r2: "v22 \<in> \<lbrakk>e2\<rbrakk>\<rho>2" and
+      v12_n3: "v12 <: TNat n3" and v22_n4: "v22 <: TNat n4" and
+      fn34_v2: "TNat (f n3 n4) <: v2" and wf_v2: "wf_ty v2" using v2_p by auto
+        
+    have IH1: "determ v11 v12 e1 \<rho>1 \<rho>2" using EPrim(1) by simp
+    have "wf_ty (v11 \<sqinter> v12)" using IH1 v11_e1_r1 v12_e1_r2 c_r1_r2 wf_r1 wf_r2 by blast
+    then have "TNat n1 ~ TNat n3" using v11_n1 v12_n3 consis_le by blast
+    then have n1_n3: "n1 = n3" by simp
+        
+    have IH2: "determ v21 v22 e2 \<rho>1 \<rho>2" using EPrim(2) by simp
+    have "wf_ty (v21 \<sqinter> v22)" using IH2 v21_e2_r1 v22_e2_r2 c_r1_r2 wf_r1 wf_r2 by blast
+    then have "TNat n2 ~ TNat n4" using v21_n2 v22_n4 consis_le by blast
+    then have n2_n4: "n2 = n4" by simp
+        
+    have v1_v2: "v1 ~ v2" using n1_n3 n2_n4 fn12_v1 fn34_v2 consis_le by blast
+    have r12_r1: "\<rho>1\<sqinter>\<rho>2 <: \<rho>1" using c_r1_r2 apply auto done
+        
+    have v11_r12: "v11 \<in> \<lbrakk>e1\<rbrakk>\<rho>1\<sqinter>\<rho>2" using r12_r1 v11_e1_r1 weaken_env by blast
+    have v21_r12: "v21 \<in> \<lbrakk>e2\<rbrakk>\<rho>1\<sqinter>\<rho>2" using r12_r1 v21_e2_r1 weaken_env by blast
+        
+    show "v1 \<sqinter> v2 \<in> \<lbrakk>EPrim f e1 e2\<rbrakk>\<rho>1 \<sqinter> \<rho>2 \<and> wf_ty (v1 \<sqinter> v2)"
+      using v11_r12 v21_r12 v1_v2 wf_v1 wf_v2
+      apply simp using fn12_v1 fn34_v2 n1_n3 n2_n4 v11_n1 v21_n2 by blast
+  qed
+next
+  case (EIf e1 e2 e3)
+  show ?case
+    apply (rule allI)+ apply (rule impI)+
+  proof -
+    fix v1 v2 \<rho>1 \<rho>2
+    assume v1_p: "v1 \<in> \<lbrakk>EIf e1 e2 e3\<rbrakk>\<rho>1" and v2_p: "v2 \<in> \<lbrakk>EIf e1 e2 e3\<rbrakk>\<rho>2" and 
+      wf_r1: "wf_env \<rho>1" and wf_r2: "wf_env \<rho>2" and c_r1_r2: "consis_env \<rho>1 \<rho>2"
+    obtain v11 n1 where v11_e1: "v11 \<in> \<lbrakk>e1\<rbrakk>\<rho>1" and v11_n1: "v11 <: TNat n1" and
+      v1_e3: "n1 = 0 \<longrightarrow> v1 \<in> \<lbrakk>e3\<rbrakk>\<rho>1" and v1_e2: "n1 \<noteq> 0 \<longrightarrow> v1 \<in> \<lbrakk>e2\<rbrakk>\<rho>1" using v1_p by auto
+    obtain v12 n2 where v12_e1: "v12 \<in> \<lbrakk>e1\<rbrakk>\<rho>2" and v12_n2: "v12 <: TNat n2" and
+      v2_e3: "n2 = 0 \<longrightarrow> v2 \<in> \<lbrakk>e3\<rbrakk>\<rho>2" and v2_e2: "n2 \<noteq> 0 \<longrightarrow> v2 \<in> \<lbrakk>e2\<rbrakk>\<rho>2" using v2_p by auto
+        
+    have IH1: "determ v11 v12 e1 \<rho>1 \<rho>2" using EIf(1) by simp
+    have "wf_ty (v11 \<sqinter> v12)" using IH1 v11_e1 v12_e1 c_r1_r2 wf_r1 wf_r2 by blast
+    then have "TNat n1 ~ TNat n2" using v11_n1 v12_n2 consis_le by blast
+    then have n1_n2: "n1 = n2" by simp
+        
+    have IH2: "determ v1 v2 e2 \<rho>1 \<rho>2" using EIf(2) by simp
+    have IH3: "determ v1 v2 e3 \<rho>1 \<rho>2" using EIf(3) by simp
+        
+    { assume n1: "n1 = 0"
+      have "v1 \<sqinter> v2 \<in> \<lbrakk>e3\<rbrakk>\<rho>1\<sqinter>\<rho>2" and "wf_ty (v1 \<sqinter> v2)"
+        using IH3 v1_e3 v2_e3 wf_r1 wf_r2 c_r1_r2 wf_r1 wf_r2 n1 n1_n2 by auto
+    } moreover { assume n1: "n1 \<noteq> 0"
+      have "v1 \<sqinter> v2 \<in> \<lbrakk>e2\<rbrakk>\<rho>1\<sqinter>\<rho>2" and "wf_ty (v1 \<sqinter> v2)"
+        using IH2 v1_e2 v2_e2 wf_r1 wf_r2 c_r1_r2 wf_r1 wf_r2 n1 n1_n2 by auto        
+    } ultimately
+    show "v1 \<sqinter> v2 \<in> \<lbrakk>EIf e1 e2 e3\<rbrakk>\<rho>1 \<sqinter> \<rho>2 \<and> wf_ty (v1 \<sqinter> v2)"
+      by (smt E.simps(6) c_r1_r2 case_prod_conv length_map length_zip mem_Collect_eq
+          min.idem n1_n2 nth_map nth_zip sub_inter_right2 sub_refl v12_e1 v12_n2 weaken_env)          
+  qed
+qed    
+
+section "Subsumption is Admissible"  
+
+lemma fun_eval_distr:
+  "\<lbrakk> F (A \<rightarrow> B \<sqinter> C \<rightarrow> D) e \<rho>; wf_env \<rho>; wf_ty A; wf_ty C; A ~ C \<rbrakk>
+    \<Longrightarrow> F ((A \<sqinter> C) \<rightarrow> (B \<sqinter> D)) e \<rho>"
+  apply simp apply clarify
+  apply (subgoal_tac "(A\<sqinter>C)#\<rho> <: A # \<rho>") prefer 2 apply simp 
+   apply clarify apply (case_tac k) apply force apply force
+  apply (subgoal_tac "(A\<sqinter>C)#\<rho> <: C # \<rho>") prefer 2 apply simp 
+   apply clarify apply (case_tac k) apply force apply force
+  apply (subgoal_tac "B \<in> \<lbrakk>e\<rbrakk>(A\<sqinter>C)#\<rho>") prefer 2 using weaken_env apply blast
+  apply (subgoal_tac "D \<in> \<lbrakk>e\<rbrakk>(A\<sqinter>C)#\<rho>") prefer 2 using weaken_env apply blast
+  apply (subgoal_tac "wf_env ((A\<sqinter>C)#\<rho>)") prefer 2 apply simp apply clarify
+    apply (case_tac k) apply simp apply blast apply force
+  apply (subgoal_tac "B \<sqinter> D \<in> \<lbrakk>e\<rbrakk>((A \<sqinter> C) # \<rho>) \<sqinter> ((A \<sqinter> C) # \<rho>)") prefer 2 
+    using deterministic consis_refl apply presburger
+  apply (subgoal_tac "(A \<sqinter> C) # \<rho> <: ((A \<sqinter> C) # \<rho>) \<sqinter> ((A \<sqinter> C) # \<rho>)") prefer 2
+   apply simp apply clarify apply (case_tac k) prefer 2 apply force
+    apply simp 
+  apply blast
+  apply (rule weaken_env)    
+   apply blast
+    apply blast
+  done
+
 lemma denot_fun_fold_meet:
   "\<lbrakk> F (fold op \<sqinter> L (A\<rightarrow>B)) e \<rho>; all_funs (set L); wf_env \<rho>; wf_ty A; wf_ty B;
-     wf_list L; consis_funs ((A\<rightarrow>B)#L);
-     \<forall>v1 v2 \<rho>1 \<rho>2. determ v1 v2 e \<rho>1 \<rho>2 \<rbrakk> \<Longrightarrow> 
+     wf_list L; consis_funs ((A\<rightarrow>B)#L) \<rbrakk> \<Longrightarrow> 
     F ((fold op \<sqinter> (map dom L) A) \<rightarrow> (fold op \<sqinter> (map cod L) B)) e \<rho>"
   apply (induction L arbitrary: A B)
    apply force
@@ -250,17 +415,18 @@ lemma denot_fun_fold_meet:
   apply (subgoal_tac "F (fold op \<sqinter> L ((A'\<sqinter>A) \<rightarrow> (B' \<sqinter> B))) e \<rho>") prefer 2
    apply (rule denot_fold_meet_swap_init)
     apply force
-   apply (rule fun_eval_distr_determ)
+   apply (rule fun_eval_distr)
    apply (subgoal_tac "F (A' \<rightarrow> B' \<sqinter> A \<rightarrow> B) e \<rho>") prefer 2
          apply (rule denot_fold_meet_inv_init)
          apply force
-   apply assumption apply assumption apply assumption 
+   apply assumption apply assumption 
    apply force
     apply assumption
   apply (metis bot_least consis_sym insert_mono list.set(2))
   apply (subgoal_tac "wf_ty (A'\<sqinter>A)") 
    apply (subgoal_tac "wf_ty (B'\<sqinter>B)")
-   apply (subgoal_tac "\<forall>v1 v1' v2 v2'. {v1\<rightarrow>v1',v2\<rightarrow>v2'} \<subseteq> insert ((A'\<sqinter>A)\<rightarrow>(B'\<sqinter>B)) (set L) \<longrightarrow> v1 ~ v2 \<and> v1' ~ v2'")
+    apply (subgoal_tac "\<forall>v1 v1' v2 v2'. {v1\<rightarrow>v1',v2\<rightarrow>v2'} \<subseteq> insert ((A'\<sqinter>A)\<rightarrow>(B'\<sqinter>B)) (set L)
+                         \<longrightarrow> v1 ~ v2 \<and> v1' ~ v2'")
      apply simp
     defer
       
@@ -322,11 +488,10 @@ proof -
       show ?thesis using v11 v22 1 apply auto done
     qed 
   qed    
-qed
+qed    
   
 lemma denot_fun_meet_list: "\<lbrakk> F (\<Sqinter>L) e \<rho>; L \<noteq> []; all_funs (set L); wf_env \<rho>;
-   consis_funs L; wf_list L;
-   \<forall> v1 v2 \<rho>1 \<rho>2. determ v1 v2 e \<rho>1 \<rho>2 \<rbrakk> 
+   consis_funs L; wf_list L \<rbrakk> 
   \<Longrightarrow> F (\<Sqinter>(map dom L) \<rightarrow> \<Sqinter>(map cod L)) e \<rho>"
   apply (cases L) apply force
   unfolding meet_list_def apply clarify
@@ -335,12 +500,14 @@ lemma denot_fun_meet_list: "\<lbrakk> F (\<Sqinter>L) e \<rho>; L \<noteq> []; a
   apply (subgoal_tac "wf_ty x22") prefer 2 apply blast    
     using denot_fun_fold_meet apply simp 
   done
+
+abbreviation subsump :: "ty \<Rightarrow> ty \<Rightarrow> exp \<Rightarrow> ty list \<Rightarrow> bool" where
+  "subsump v1 v2 e \<rho> \<equiv> v1 \<in> \<lbrakk>e\<rbrakk>\<rho> \<longrightarrow> v1 <: v2 \<longrightarrow> wf_ty v2 \<longrightarrow> wf_env \<rho> \<longrightarrow> v2 \<in> \<lbrakk>e\<rbrakk>\<rho>" 
     
 lemma subsumption_fun: fixes v1::ty and v2::ty
   assumes v1_e: "F v1 e \<rho>" and v1_v2: "v1 <: v2" and
     wf_v1: "wf_ty v1"  and wf_v2: "wf_ty v2" and wf_r: "wf_env \<rho>" and
-    IH: "\<forall>v1 v2 \<rho>. subsump v1 v2 e \<rho>" and
-    D: "\<forall> v1 v2 \<rho>1 \<rho>2. determ v1 v2 e \<rho>1 \<rho>2"
+    IH: "\<forall>v1 v2 \<rho>. subsump v1 v2 e \<rho>"
   shows "F v2 e \<rho>"
 proof (rule denot_fun_atoms)
   have "all_funs (atoms v1)" using v1_e eval_fun_all_funs by simp
@@ -378,7 +545,7 @@ next
         apply (case_tac xa) apply auto done
       then have "F (\<Sqinter>\<Gamma>1) e \<rho>" using v1_e_atoms af_mg1 denot_fun_atoms by blast
       then have "F (\<Sqinter>(map dom \<Gamma>1) \<rightarrow> \<Sqinter>(map cod \<Gamma>1)) e \<rho>"
-        using denot_fun_meet_list D af_g g_ne wf_r c_g1 wf_g1 by blast
+        using denot_fun_meet_list af_g g_ne wf_r c_g1 wf_g1 by blast
       then have cg1_e: "\<Sqinter> (map cod \<Gamma>1) \<in> \<lbrakk>e\<rbrakk>(\<Sqinter> (map dom \<Gamma>1))#\<rho>" by simp
       have "A#\<rho> <: (\<Sqinter> (map dom \<Gamma>1))#\<rho>" using a_dg apply auto apply (case_tac k) apply auto done
       then have cg1_e: "\<Sqinter> (map cod \<Gamma>1) \<in> \<lbrakk>e\<rbrakk>A#\<rho>" using cg1_e weaken_env by blast
@@ -389,194 +556,44 @@ next
   qed
 qed
   
-lemma subsumption_deterministic:
-  "(\<forall> v1 v2 \<rho>. subsump v1 v2 e \<rho>) \<and> (\<forall> v1 v2 \<rho>1 \<rho>2. determ v1 v2 e \<rho>1 \<rho>2)"
+lemma subsumption: "\<forall> v1 v2 \<rho>. subsump v1 v2 e \<rho>"
 proof (induction e)
   case (EVar x)
   show ?case
-  proof
-    show "\<forall>v1 v2 \<rho>. subsump v1 v2 (EVar x) \<rho>" apply clarify
-      apply (case_tac "x < length \<rho>") defer apply force
-      apply simp apply (rule sub_trans) apply auto done
-  next
-    show "\<forall>v1 v2 \<rho>1 \<rho>2. determ v1 v2 (EVar x) \<rho>1 \<rho>2" apply clarify
-      apply (case_tac "x < length \<rho>1") defer apply force
-      using consis_le inter_func by auto
-  qed
+    apply clarify
+    apply (case_tac "x < length \<rho>") defer apply force
+    apply simp apply (rule sub_trans) apply auto done
 next
   case (ENat n)
   then show ?case apply auto
-    using sub_trans apply blast
-    by (simp add: consis_le inter_func)      
+    using sub_trans apply blast done
 next
   case (ELam e)
   show ?case
-  proof
-    show "\<forall>v1 v2 \<rho>. subsump v1 v2 (\<lambda> e) \<rho>" 
       apply clarify apply simp
        apply (rule subsumption_fun) apply blast apply blast apply blast 
-         apply blast apply blast using ELam.IH apply auto done
-  next
-    show "\<forall>v1 v2 \<rho>1 \<rho>2. determ v1 v2 (\<lambda> e) \<rho>1 \<rho>2 " apply (rule allI)+ apply (rule impI)+
-    proof -
-      fix v1 v2 \<rho>1 \<rho>2 assume v1_le: "v1 \<in> \<lbrakk>\<lambda> e\<rbrakk>\<rho>1" and v2_le: "v2 \<in> \<lbrakk>\<lambda> e\<rbrakk>\<rho>2" and
-        wf_r1: "wf_env \<rho>1" and wf_r2: "wf_env \<rho>2" and c_r1_r2: "consis_env \<rho>1 \<rho>2" 
-      have wf_v1: "wf_ty v1" using v1_le by simp
-      have wf_v2: "wf_ty v2" using v2_le by simp
-      have f_v1_e_r1: "F v1 e \<rho>1" using v1_le by simp      
-      have f_v2_e_r2: "F v2 e \<rho>2" using v2_le by simp      
-      have r12_r1: "\<rho>1\<sqinter>\<rho>2 <: \<rho>1" using c_r1_r2 by auto
-      have r12_r2: "\<rho>1\<sqinter>\<rho>2 <: \<rho>2" using c_r1_r2 by auto
-      have "v1 ~ v2" apply (rule atoms_consis) apply clarify
-      proof -
-        fix A1 A2 assume a1_v1: "A1 \<in> atoms v1" and a2_v2: "A2 \<in> atoms v2"
-        obtain A11 A12 where a1: "A1=A11\<rightarrow>A12" and a12_e: "A12 \<in> \<lbrakk>e\<rbrakk>A11#\<rho>1" using f_v1_e_r1 
-          by (metis a1_v1 atoms_not_inter denot_fun_inv_atoms ty.simps(10) wf_atoms wf_ty.simps wf_v1)
-        obtain A21 A22 where a2: "A2=A21\<rightarrow>A22" and a22_e: "A22 \<in> \<lbrakk>e\<rbrakk>A21#\<rho>2" using f_v2_e_r2 
-          by (metis a2_v2 atoms_not_inter denot_fun_inv_atoms ty.simps(10) wf_atoms wf_ty.simps wf_v2)
-        show "A1 ~ A2"
-        proof (cases "A11 ~ A21")
-          case True
-          have c_ar1_ar2: "consis_env (A11#\<rho>1) (A21#\<rho>2)" using True c_r1_r2 apply auto
-              apply (case_tac k) apply auto done
-          have wf_ar1: "wf_env (A11#\<rho>1)" using wf_r1 a1 a1_v1 wf_v1 apply auto
-              apply (case_tac k) apply auto using wf_ty_arrow_inv by blast
-          have wf_ar2: "wf_env (A21#\<rho>2)" using wf_r2 a2 a2_v2 wf_v2 apply auto
-            apply (case_tac k) apply auto using wf_ty_arrow_inv by blast
-          have "determ A12 A22 e (A11#\<rho>1) (A21#\<rho>2)" using ELam by blast
-          then show ?thesis using c_ar1_ar2 a12_e a22_e wf_ar1 wf_ar2 True a1 a2 by auto
-        next
-          case False
-          then show ?thesis using a1 a2 by simp
-        qed
-      qed        
-      then have wf_v12: "wf_ty (v1 \<sqinter> v2)" using wf_v1 wf_v2 by auto
-      have f_v1_e: "F v1 e (\<rho>1 \<sqinter> \<rho>2)" using f_v1_e_r1 r12_r1 weaken_env_fun by blast
-      have f_v2_e: "F v2 e (\<rho>1 \<sqinter> \<rho>2)" using f_v2_e_r2 r12_r2 weaken_env_fun by blast
-      show "v1 \<sqinter> v2 \<in> \<lbrakk>\<lambda> e\<rbrakk>\<rho>1 \<sqinter> \<rho>2 \<and> wf_ty (v1 \<sqinter> v2)" using wf_v12 f_v1_e f_v2_e by simp
-    qed
-  qed
+         apply blast apply blast using ELam.IH deterministic apply auto done
 next
   case (EApp e1 e2)
   show ?case
-  proof
-    show "\<forall>v1 v2 \<rho>. subsump v1 v2 (EApp e1 e2) \<rho>"
-      apply clarify apply simp apply clarify
-    proof -
-      fix v1::ty and v2 \<rho> f v assume v1_v2: "v1 <: v2" and wf_v2: "wf_ty v2" and wf_r: "wf_env \<rho>" and
-        f_e1: "f \<in> \<lbrakk>e1\<rbrakk>\<rho>" and v_e2: "v \<in> \<lbrakk>e2\<rbrakk>\<rho>" and f_vv1: "f <: v \<rightarrow> v1" and wf_v1: "wf_ty v1"
-      have "v \<rightarrow> v1 <: v \<rightarrow> v2" using v1_v2 by blast
-      then have "f <: v \<rightarrow> v2" using f_vv1 sub_trans by blast
-      then show "\<exists>f. f \<in> \<lbrakk>e1\<rbrakk>\<rho> \<and> (\<exists>v. v \<in> \<lbrakk>e2\<rbrakk>\<rho> \<and> f <: v \<rightarrow> v2)" 
-        using f_e1 v_e2 by blast
-    qed
-  next
-    show "\<forall>v1 v2 \<rho>1 \<rho>2. determ v1 v2 (EApp e1 e2) \<rho>1 \<rho>2 "
-      apply (rule allI)+ apply (rule impI)+
-    proof -
-      fix v1 v2 \<rho>1 \<rho>2 assume v1_e1e2: "v1 \<in> \<lbrakk>EApp e1 e2\<rbrakk>\<rho>1" and v2_e1e2: "v2 \<in> \<lbrakk>EApp e1 e2\<rbrakk>\<rho>2" and
-        wf_r1: "wf_env \<rho>1" and wf_r2: "wf_env \<rho>2" and c_r1_r2: "consis_env \<rho>1 \<rho>2"
-      obtain f1 v21 where f1_e1: "f1 \<in> \<lbrakk>e1\<rbrakk>\<rho>1" and v21_e2: "v21\<in> \<lbrakk>e2\<rbrakk>\<rho>1" and f1_v21: "v1 \<in> f1 \<bullet> v21" 
-        using v1_e1e2 by auto
-      obtain f2 v22 where f2_e1: "f2 \<in> \<lbrakk>e1\<rbrakk>\<rho>2" and v22_e2: "v22\<in> \<lbrakk>e2\<rbrakk>\<rho>2" and f2_v22: "v2 \<in> f2 \<bullet> v22" 
-        using v2_e1e2 by auto
-      have "determ f1 f2 e1 \<rho>1 \<rho>2" using EApp(1) by blast
-      then have f12_e1: "f1 \<sqinter> f2 \<in> \<lbrakk>e1\<rbrakk>\<rho>1\<sqinter>\<rho>2" and wf_f12: "wf_ty (f1 \<sqinter> f2)"         
-        using f1_e1 f2_e1 wf_r1 wf_r2 c_r1_r2 by auto
-      have "determ v21 v22 e2 \<rho>1 \<rho>2" using EApp(2) by blast
-      then have v22_e2: "v21 \<sqinter> v22 \<in> \<lbrakk>e2\<rbrakk>\<rho>1\<sqinter>\<rho>2" and wf_v21_v22: "wf_ty (v21 \<sqinter> v22)"
-        using v21_e2 v22_e2 wf_r1 wf_r2 c_r1_r2 by auto
-      have f12_v21_v22: "v1 \<sqinter> v2 \<in> (f1 \<sqinter> f2) \<bullet> (v21 \<sqinter> v22)"
-        using inter_app[of v1 f1 v21 v2 f2 v22] f1_v21 f2_v22 wf_f12 wf_v21_v22 
-        by (metis CollectD consis_le consistent.simps(4) wf_ty_inter_inv)
-      have v1_v2: "v1 ~ v2"
-        using consistent_app[of f1 f2 v21 v22 v1 v2] wf_f12 wf_v21_v22 f1_v21 f2_v22 by blast
-      have wf_v1: "wf_ty v1" using f1_v21 by blast
-      have wf_v2: "wf_ty v2" using f2_v22 by blast
-      show "v1 \<sqinter> v2 \<in> \<lbrakk>EApp e1 e2\<rbrakk>\<rho>1 \<sqinter> \<rho>2 \<and> wf_ty (v1 \<sqinter> v2)"
-        using f12_e1 v22_e2 v1_v2 wf_v1 wf_v2 v1_v2 f12_v21_v22 by auto
-    qed      
-  qed    
-next
-  case (EPrim f e1 e2)
-  show ?case 
-  proof
-    show "\<forall>v1 v2 \<rho>. subsump v1 v2 (EPrim f e1 e2) \<rho>" apply simp by (meson sub_trans)
-  next
-    show "\<forall>v1 v2 \<rho>1 \<rho>2. determ v1 v2 (EPrim f e1 e2) \<rho>1 \<rho>2" 
-      apply (rule allI)+ apply (rule impI)+
-    proof -
-      fix v1 v2 \<rho>1 \<rho>2
-      assume v1_p: "v1 \<in> \<lbrakk>EPrim f e1 e2\<rbrakk>\<rho>1" and v2_p: "v2 \<in> \<lbrakk>EPrim f e1 e2\<rbrakk>\<rho>2" and 
-        wf_r1: "wf_env \<rho>1" and wf_r2: "wf_env \<rho>2" and c_r1_r2: "consis_env \<rho>1 \<rho>2"
-      obtain v11 v21 n1 n2 where v11_e1_r1: "v11 \<in> \<lbrakk>e1\<rbrakk>\<rho>1" and v21_e2_r1: "v21 \<in> \<lbrakk>e2\<rbrakk>\<rho>1" and
-        v11_n1: "v11 <: TNat n1" and v21_n2: "v21 <: TNat n2" and
-        fn12_v1: "TNat (f n1 n2) <: v1" and wf_v1: "wf_ty v1" using v1_p by auto
-      obtain v12 v22 n3 n4 where v12_e1_r2: "v12 \<in> \<lbrakk>e1\<rbrakk>\<rho>2" and v22_e2_r2: "v22 \<in> \<lbrakk>e2\<rbrakk>\<rho>2" and
-        v12_n3: "v12 <: TNat n3" and v22_n4: "v22 <: TNat n4" and
-        fn34_v2: "TNat (f n3 n4) <: v2" and wf_v2: "wf_ty v2" using v2_p by auto
-
-      have IH1: "determ v11 v12 e1 \<rho>1 \<rho>2" using EPrim(1) by simp
-      have "wf_ty (v11 \<sqinter> v12)" using IH1 v11_e1_r1 v12_e1_r2 c_r1_r2 wf_r1 wf_r2 by blast
-      then have "TNat n1 ~ TNat n3" using v11_n1 v12_n3 consis_le by blast
-      then have n1_n3: "n1 = n3" by simp
-          
-      have IH2: "determ v21 v22 e2 \<rho>1 \<rho>2" using EPrim(2) by simp
-      have "wf_ty (v21 \<sqinter> v22)" using IH2 v21_e2_r1 v22_e2_r2 c_r1_r2 wf_r1 wf_r2 by blast
-      then have "TNat n2 ~ TNat n4" using v21_n2 v22_n4 consis_le by blast
-      then have n2_n4: "n2 = n4" by simp
-      
-      have v1_v2: "v1 ~ v2" using n1_n3 n2_n4 fn12_v1 fn34_v2 consis_le by blast
-      have r12_r1: "\<rho>1\<sqinter>\<rho>2 <: \<rho>1" using c_r1_r2 apply auto done
-          
-      have v11_r12: "v11 \<in> \<lbrakk>e1\<rbrakk>\<rho>1\<sqinter>\<rho>2" using r12_r1 v11_e1_r1 weaken_env by blast
-      have v21_r12: "v21 \<in> \<lbrakk>e2\<rbrakk>\<rho>1\<sqinter>\<rho>2" using r12_r1 v21_e2_r1 weaken_env by blast
-          
-      show "v1 \<sqinter> v2 \<in> \<lbrakk>EPrim f e1 e2\<rbrakk>\<rho>1 \<sqinter> \<rho>2 \<and> wf_ty (v1 \<sqinter> v2)"
-        using v11_r12 v21_r12 v1_v2 wf_v1 wf_v2
-          apply simp using fn12_v1 fn34_v2 n1_n3 n2_n4 v11_n1 v21_n2 by blast
-    qed
+    apply clarify apply simp apply clarify
+  proof -
+    fix v1::ty and v2 \<rho> f v assume v1_v2: "v1 <: v2" and 
+      wf_v1: "wf_ty v1" and wf_v2: "wf_ty v2" and wf_r: "wf_env \<rho>" and
+      f_e1: "f \<in> \<lbrakk>e1\<rbrakk>\<rho>" and v_e2: "v \<in> \<lbrakk>e2\<rbrakk>\<rho>" and f_vv1: "f <: v \<rightarrow> v1" 
+    have "v \<rightarrow> v1 <: v \<rightarrow> v2" using v1_v2 by blast
+    then have "f <: v \<rightarrow> v2" using f_vv1 sub_trans by blast
+    then show "\<exists>f. f \<in> \<lbrakk>e1\<rbrakk>\<rho> \<and> (\<exists>v. v \<in> \<lbrakk>e2\<rbrakk>\<rho> \<and> f <: v \<rightarrow> v2)" 
+      using f_e1 v_e2 by blast
   qed
 next
+  case (EPrim f e1 e2)
+  show ?case apply simp by (meson sub_trans)
+next
   case (EIf e1 e2 e3)
-  show ?case
-  proof
-    show "\<forall>v1 v2 \<rho>. subsump v1 v2 (EIf e1 e2 e3) \<rho>"
-      apply simp  by (meson EIf.IH(2) EIf.IH(3))
-  next
-    show "\<forall>v1 v2 \<rho>1 \<rho>2. determ v1 v2 (EIf e1 e2 e3) \<rho>1 \<rho>2" 
-      apply (rule allI)+ apply (rule impI)+
-    proof -
-      fix v1 v2 \<rho>1 \<rho>2
-      assume v1_p: "v1 \<in> \<lbrakk>EIf e1 e2 e3\<rbrakk>\<rho>1" and v2_p: "v2 \<in> \<lbrakk>EIf e1 e2 e3\<rbrakk>\<rho>2" and 
-        wf_r1: "wf_env \<rho>1" and wf_r2: "wf_env \<rho>2" and c_r1_r2: "consis_env \<rho>1 \<rho>2"
-      obtain v11 n1 where v11_e1: "v11 \<in> \<lbrakk>e1\<rbrakk>\<rho>1" and v11_n1: "v11 <: TNat n1" and
-         v1_e3: "n1 = 0 \<longrightarrow> v1 \<in> \<lbrakk>e3\<rbrakk>\<rho>1" and v1_e2: "n1 \<noteq> 0 \<longrightarrow> v1 \<in> \<lbrakk>e2\<rbrakk>\<rho>1" using v1_p by auto
-      obtain v12 n2 where v12_e1: "v12 \<in> \<lbrakk>e1\<rbrakk>\<rho>2" and v12_n2: "v12 <: TNat n2" and
-         v2_e3: "n2 = 0 \<longrightarrow> v2 \<in> \<lbrakk>e3\<rbrakk>\<rho>2" and v2_e2: "n2 \<noteq> 0 \<longrightarrow> v2 \<in> \<lbrakk>e2\<rbrakk>\<rho>2" using v2_p by auto
-          
-      have IH1: "determ v11 v12 e1 \<rho>1 \<rho>2" using EIf(1) by simp
-      have "wf_ty (v11 \<sqinter> v12)" using IH1 v11_e1 v12_e1 c_r1_r2 wf_r1 wf_r2 by blast
-      then have "TNat n1 ~ TNat n2" using v11_n1 v12_n2 consis_le by blast
-      then have n1_n2: "n1 = n2" by simp
-      
-      have IH2: "determ v1 v2 e2 \<rho>1 \<rho>2" using EIf(2) by simp
-      have IH3: "determ v1 v2 e3 \<rho>1 \<rho>2" using EIf(3) by simp
-      
-      { assume n1: "n1 = 0"
-        have "v1 \<sqinter> v2 \<in> \<lbrakk>e3\<rbrakk>\<rho>1\<sqinter>\<rho>2" and "wf_ty (v1 \<sqinter> v2)"
-          using IH3 v1_e3 v2_e3 wf_r1 wf_r2 c_r1_r2 wf_r1 wf_r2 n1 n1_n2 by auto
-      } moreover { assume n1: "n1 \<noteq> 0"
-        have "v1 \<sqinter> v2 \<in> \<lbrakk>e2\<rbrakk>\<rho>1\<sqinter>\<rho>2" and "wf_ty (v1 \<sqinter> v2)"
-          using IH2 v1_e2 v2_e2 wf_r1 wf_r2 c_r1_r2 wf_r1 wf_r2 n1 n1_n2 by auto        
-      } ultimately
-      show "v1 \<sqinter> v2 \<in> \<lbrakk>EIf e1 e2 e3\<rbrakk>\<rho>1 \<sqinter> \<rho>2 \<and> wf_ty (v1 \<sqinter> v2)"
-        by (smt E.simps(6) c_r1_r2 case_prod_conv length_map length_zip mem_Collect_eq
-            min.idem n1_n2 nth_map nth_zip sub_inter_right2 sub_refl v12_e1 v12_n2 weaken_env)          
-    qed
-  qed    
+  show ?case apply simp by (meson EIf.IH(2) EIf.IH(3))
 qed  
-  
+
 (*<*)
 end
 (*>*)
